Add conditions + Stdlib Improvement (wip)

translator/lib/Ast.ml
@@ -5,4 +5,4 @@ type expr =
 (* A file is a list of bindings.
    [ [let a = e; ...] ] is translated by [ [ (Some "a", «translation of e») ]; ... ].
    The [None] case is used when unit or PAny appear. *)
-type ast = (string option * expr) list
+type ast = (string option * bool * expr) list
