theories/libs/Stdlib.v
@@ -11,58 +11,126 @@ From osiris.lang Require Import lang.
 From osiris.semantics Require Import semantics.
 From osiris.weakestpre Require Import wp wp_tactics notations.
 
-Section StdLib.
+(* The symbols of the OCaml standard library are translated as
+   [Stdlib.<symbol>].
+   This file defines:
+     1. symbols of [Stdlib], eg. (+), ... ;
+     2. [Stdlib] as a module ;
+     3.a. specifications for the symbols of the module ;
+     3.b. a unified specification for the module ;
+     4. a tactic to use automatically apply the aforementioned specs.
+
+   After 3.b., the code is turned opaque to (1) better control its usage and (2)
+   avoid it to be unfolded: some unfolding would lead to several duplications of
+   continuations (ie. the rest of the code). *)
+
+Section StdLib__code.
   Context `{!osirisGS_gen hlc Σ}.
 
-  (* About integers. *)
-  Definition Stdlib__add : val :=
-    VClo EnvNil $
-      AnonFun "x" $
-      EAnonFun $ AnonFun "y" $
-      EIntAdd (EVar "x") (EVar "y").
-  Definition Stdlib__sub : val :=
-    VClo EnvNil $
-      AnonFun "x" $
-      EAnonFun $ AnonFun "y" $
-      EIntSub (EVar "x") (EVar "y").
+  Section Arithmetic_operations.
+    Definition Stdlib__add : val :=
+      VClo EnvNil $
+           AnonFun "x" $
+           EAnonFun $ AnonFun "y" $
+           EIntAdd (EVar "x") (EVar "y").
+    Definition Stdlib__sub : val :=
+      VClo EnvNil $
+           AnonFun "x" $
+           EAnonFun $ AnonFun "y" $
+           EIntSub (EVar "x") (EVar "y").
+    Definition Stdlib__mul : val :=
+      VClo EnvNil $
+           AnonFun "x" $
+           EAnonFun $ AnonFun "y" $
+           EIntMul (EVar "x") (EVar "y").
+    Definition Stdlib__div : val :=
+      VClo EnvNil $
+           AnonFun "x" $
+           EAnonFun $ AnonFun "y" $
+           EIntDiv (EVar "x") (EVar "y").
+    Definition Stdlib__mod : val :=
+      VClo EnvNil $
+           AnonFun "x" $
+           EAnonFun $ AnonFun "y" $
+           EIntMod (EVar "x") (EVar "y").
 
 
-  (* About references. *)
-  Definition Stdlib__ref : val :=
-    VClo EnvNil $
-      AnonFun "e" $
-      ERef (EVar "e").
-
-  Definition Stdlib__load : val :=
-    VClo EnvNil $
-      AnonFun "x" $
-      ELoad (EVar "x").
-
-  Definition Stdlib__store : val :=
-    VClo EnvNil $
-      AnonFun "x" $
-      EAnonFun $ AnonFun "i" $
-      EStore (EVar "x") (EVar "i").
+    Definition Stdlib__neg : val :=
+      VClo EnvNil $
+           AnonFun "x" $
+           EIntNeg (EVar "x").
+  End Arithmetic_operations.
 
 
-  (* About tuples *)
-  Definition Stdlib__fst : val :=
-    VClo EnvNil $
-      AnonFun "x" $
-      EMatch
-        (EVar "x")
-        (BrCons
-           (Branch (PTuple (PCons (PVar "l") (PCons (PVar "r") PNil))) (EVar "l"))
-        BrNil).
 
-  Definition Stdlib__snd : val :=
-    VClo EnvNil $
-      AnonFun "x" $
-      EMatch
-        (EVar "x")
-        (BrCons
-           (Branch (PTuple (PCons (PVar "l") (PCons (PVar "r") PNil))) (EVar "r"))
-        BrNil).
+  Section Arithmetic_comparison.
+    Definition Stdlib__eq : val :=
+      VClo EnvNil $
+           AnonFun "x" $
+           EAnonFun $ AnonFun "y" $
+           EOpEq (EVar "x") (EVar "y").
+    Definition Stdlib__lt : val :=
+      VClo EnvNil $
+           AnonFun "x" $
+           EAnonFun $ AnonFun "y" $
+           EOpLt (EVar "x") (EVar "y").
+    Definition Stdlib__ge : val :=
+      VClo EnvNil $
+           AnonFun "x" $
+           EAnonFun $ AnonFun "y" $
+           EOpGe (EVar "x") (EVar "y").
+    Definition Stdlib__gt : val :=
+      VClo EnvNil $
+           AnonFun "x" $
+           EAnonFun $ AnonFun "y" $
+           EOpGt (EVar "x") (EVar "y").
+  End Arithmetic_comparison.
+
+
+
+  Section Stdlib__store.
+    Definition Stdlib__ref : val :=
+      VClo EnvNil $
+           AnonFun "e" $
+           ERef (EVar "e").
+
+    Definition Stdlib__load : val :=
+      VClo EnvNil $
+           AnonFun "x" $
+           ELoad (EVar "x").
+
+    Definition Stdlib__store : val :=
+      VClo EnvNil $
+           AnonFun "x" $
+           EAnonFun $ AnonFun "i" $
+           EStore (EVar "x") (EVar "i").
+  End Stdlib__store.
+
+
+
+  Section Stdlib__tuples.
+    Definition Stdlib__fst : val :=
+      VClo EnvNil $
+           AnonFun "x" $
+           EMatch
+           (EVar "x")
+           (BrCons
+              (Branch
+                 (PTuple (PCons (PVar "l") (PCons (PVar "r") PNil)))
+                 (EVar "l"))
+              BrNil).
+
+    Definition Stdlib__snd : val :=
+      VClo EnvNil $
+           AnonFun "x" $
+           EMatch
+           (EVar "x")
+           (BrCons
+              (Branch
+                 (PTuple (PCons (PVar "l") (PCons (PVar "r") PNil)))
+                 (EVar "r"))
+              BrNil).
+  End Stdlib__tuples.
 
 
 
@@ -71,114 +139,179 @@ Section StdLib.
     VStruct $
       EnvCons "-" Stdlib__sub $
       EnvCons "+" Stdlib__add $
+      EnvCons "*" Stdlib__mul $
+      EnvCons "~-" Stdlib__neg $
+      EnvCons "=" Stdlib__eq $
+      EnvCons "<" Stdlib__lt $
+      EnvCons ">=" Stdlib__ge $
+      EnvCons ">" Stdlib__gt $
       EnvCons "ref" Stdlib__ref $
       EnvCons "!" Stdlib__load $
       EnvCons ":=" Stdlib__store $
       EnvCons "fst" Stdlib__fst $
       EnvCons "snd" Stdlib__snd $
       EnvNil.
+End StdLib__code.
 
 
 
-  (* Specifications : integers. *)
-  Lemma Stdlib__add__spec s E:
-    ∀ v1 v2 i1 i2,
-    v1 = VInt (int.repr i1) →
-    v2 = VInt (int.repr i2) →
-    ⊢ WP call Stdlib__add v1 @s; E
-         {{ λ v, WP call v v2 @s; E {{ λ v, ⌜v = VInt (int.repr (i1 + i2))⌝ }} }}.
-  Proof.
-    intros. subst. wp.
-    wp_call.
-    by rewrite int.add_repr_repr.
-  Qed.
-
-  Lemma Stdlib__sub__spec s E:
-    ∀ v1 v2 i1 i2,
-    v1 = VInt (int.repr i1) →
-    v2 = VInt (int.repr i2) →
-    ⊢ WP call Stdlib__sub v1 @s; E
-         {{ λ v, WP call v v2 @s; E {{ λ v, ⌜v = VInt (int.repr (i1 - i2))⌝ }} }}.
-  Proof.
-    intros. subst. wp.
-    wp_call.
-    by rewrite int.sub_repr_repr.
-  Qed.
-
-
-
-  (* Specifications : store. *)
-  Lemma Stdlib__ref__spec v (s: stuckness) (E: coPset) :
-    ⊢ WP call Stdlib__ref v @ s; E
-           {{ λ vl, ∃ (ℓ: loc), ℓ ↦ v ∗ ⌜vl = VLoc ℓ ⌝ }}.
-  Proof.
-    wp_call. wp_alloc l "[Hl _]".
-    iExists l.
-    iFrame.
-    iPureIntro. reflexivity.
-  Qed.
-
-  Lemma Stdlib__load__spec vl l v s E :
-    {{{ ⌜vl = VLoc l⌝ ∗ l ↦ v }}}
-      call Stdlib__load vl @ s; E
-    {{{ r, RET r; ⌜r = v⌝ ∗ l ↦ v }}}.
-  Proof.
-    iIntros (φ) "[->Hpre] Hφ".
-    wp_call.
-    wp_load "Hpre".
-    wp_use "Hφ".
-    iFrame.
-    iPureIntro. reflexivity.
-  Qed.
-
-  Lemma Stdlib__store__spec vl l v v' s E :
-    {{{ ⌜vl = VLoc l⌝ ∗ l ↦ v }}}
-      call Stdlib__store vl @ s; E
-    {{{ vstore, RET vstore;
-        WP call vstore v' @ s; E
-           {{ λ v, ⌜ v = VUnit ⌝ ∗
-                   l ↦ v' }} }}}.
-  Proof.
-    iIntros (ϕ) "[-> Hℓ] Hϕ".
-    wp_call. iApply "Hϕ". clear ϕ.
-    wp_call.
-    wp_store "Hℓ". by iSplit.
-  Qed.
-
-
-  Lemma Stdlib__fst__spec v1 v2 s E :
-    {{{ ⌜ True ⌝ }}}
-      call Stdlib__fst (VTuple (VCons v1 (VCons v2 VNil))) @ s; E
-    {{{ v, RET v; ⌜ v = v1 ⌝ }}}.
-  Proof.
-    iIntros (ϕ)"_ Hϕ".
-    wp_call.
-    wp_continue.
-    by iApply "Hϕ".
-  Qed.
-
-  Lemma Stdlib__snd__spec v1 v2 s E :
-    {{{ ⌜ True ⌝ }}}
-      call Stdlib__snd (VTuple (VCons v1 (VCons v2 VNil))) @ s; E
-    {{{ v, RET v; ⌜ v = v2 ⌝ }}}.
-  Proof.
-    iIntros (ϕ)"_ Hϕ".
-    wp_call.
-    wp_continue.
-    by iApply "Hϕ".
-  Qed.
-
-  Opaque Stdlib__sub.
-  Opaque Stdlib__add.
-  Opaque Stdlib__ref.
-  Opaque Stdlib__load.
-  Opaque Stdlib__store.
-  Opaque Stdlib__fst.
-  Opaque Stdlib__snd.
-End StdLib.
-
-Section Stdlib_Lemmas.
+Section Stdlib__specs.
   Context `{!osirisGS_gen hlc Σ}.
+
+
+  Section Stdlib__spec__arithmetic.
+    Lemma Stdlib__add__spec s E:
+      ∀ v1 v2 (i1 i2: Z),
+        v1 = encode i1 →
+        v2 = encode i2 →
+        ⊢ WP call Stdlib__add v1 @s; E
+             {{ λ v, WP call v v2 @s; E
+                        {{ λ v, ⌜v = encode (i1 + i2)%Z⌝ }} }}.
+    Proof.
+      intros. subst. wp.
+      wp_call.
+      by rewrite int.add_repr_repr.
+    Qed.
+
+    Lemma Stdlib__sub__spec s E:
+      ∀ v1 v2 (i1 i2: Z),
+        v1 = encode i1 →
+        v2 = encode i2 →
+        ⊢ WP call Stdlib__sub v1 @s; E
+             {{ λ v, WP call v v2 @s; E
+                        {{ λ v, ⌜v = encode (i1 - i2)%Z⌝ }} }}.
+    Proof.
+      intros. subst. wp.
+      wp_call.
+      by rewrite int.sub_repr_repr.
+    Qed.
+
+    Lemma Stdlib__mul__spec s E:
+      ∀ v1 v2 (i1 i2: Z),
+        v1 = encode i1 →
+        v2 = encode i2 →
+        ⊢ WP call Stdlib__mul v1 @s; E
+             {{ λ v, WP call v v2 @s; E
+                        {{ λ v, ⌜v = encode (i1 * i2)%Z⌝ }} }}.
+    Proof.
+      intros. subst. wp.
+      wp_call.
+      by rewrite int.mul_repr_repr.
+    Qed.
+
+    Lemma Stdlib__neg__spec s E:
+      ∀ v1 (i1: Z),
+        v1 = encode i1 →
+        ⊢ WP call Stdlib__neg v1 @s; E
+             {{ λ v, ⌜v = encode (- i1)%Z⌝ }}.
+    Proof.
+      intros. subst. wp.
+      wp_call. iPureIntro.
+      by rewrite int.neg_repr.
+    Qed.
+  End Stdlib__spec__arithmetic.
+
+
+
+  Section Stdlib__spec__arith_comp.
+    Lemma Stdlib__eq__spec s E :
+      ∀ v1 v2 (i1 i2: Z),
+        v1 = encode i1 →
+        v2 = encode i2 →
+        (int.min_signed ≤ i1 ≤ int.max_signed)%Z →
+        (int.min_signed ≤ i2 ≤ int.max_signed)%Z →
+        ⊢ WP call Stdlib__eq v1 @s; E
+             {{ λ v, WP call v v2 @s; E
+                        {{ λ v, ⌜v = encode (i1 =? i2)%Z⌝ }} }}.
+    Proof.
+      intros. subst. wp.
+      wp_call.
+      by rewrite int.eq_repr_repr.
+    Qed.
+
+    Lemma Stdlib__lt__spec s E :
+      ∀ v1 v2 (i1 i2: Z),
+        v1 = encode i1 →
+        v2 = encode i2 →
+        (int.min_signed ≤ i1 ≤ int.max_signed)%Z →
+        (int.min_signed ≤ i2 ≤ int.max_signed)%Z →
+        ⊢ WP call Stdlib__lt v1 @s; E
+             {{ λ v, WP call v v2 @s; E
+                        {{ λ v, ⌜v = encode (i1 <? i2)%Z⌝ }} }}.
+    Proof.
+      intros. subst. wp.
+      wp_call.
+      by rewrite int.lt_repr_repr.
+    Qed.
+  End Stdlib__spec__arith_comp.
+
+
+
+  Section Stdlib__spec__store.
+    Lemma Stdlib__ref__spec v (s: stuckness) (E: coPset) :
+      ⊢ WP call Stdlib__ref v @ s; E
+           {{ λ vl, ∃ (ℓ: loc), ℓ ↦ v ∗ ⌜vl = VLoc ℓ ⌝ }}.
+    Proof.
+      wp_call. wp_alloc l "[Hl _]".
+      iExists l.
+      iFrame.
+      iPureIntro. reflexivity.
+    Qed.
+
+    Lemma Stdlib__load__spec vl l v s E :
+      {{{ ⌜vl = VLoc l⌝ ∗ l ↦ v }}}
+        call Stdlib__load vl @ s; E
+      {{{ r, RET r; ⌜r = v⌝ ∗ l ↦ v }}}.
+    Proof.
+      iIntros (φ) "[->Hpre] Hφ".
+      wp_call.
+      wp_load "Hpre".
+      wp_use "Hφ".
+      iFrame.
+      iPureIntro. reflexivity.
+    Qed.
+
+    Lemma Stdlib__store__spec vl l v v' s E :
+      {{{ ⌜vl = VLoc l⌝ ∗ l ↦ v }}}
+        call Stdlib__store vl @ s; E
+      {{{ vstore, RET vstore;
+                  WP call vstore v' @ s; E
+                     {{ λ v, ⌜ v = VUnit ⌝ ∗
+                             l ↦ v' }} }}}.
+    Proof.
+      iIntros (ϕ) "[-> Hℓ] Hϕ".
+      wp_call. iApply "Hϕ". clear ϕ.
+      wp_call.
+      wp_store "Hℓ". by iSplit.
+    Qed.
+  End Stdlib__spec__store.
+
+
+
+  Section Stdlib__spec__tuples.
+    Lemma Stdlib__fst__spec v1 v2 s E :
+      {{{ ⌜ True ⌝ }}}
+        call Stdlib__fst (VTuple (VCons v1 (VCons v2 VNil))) @ s; E
+      {{{ v, RET v; ⌜ v = v1 ⌝ }}}.
+    Proof.
+      iIntros (ϕ)"_ Hϕ".
+      wp_call.
+      wp_continue.
+      by iApply "Hϕ".
+    Qed.
+
+    Lemma Stdlib__snd__spec v1 v2 s E :
+      {{{ ⌜ True ⌝ }}}
+        call Stdlib__snd (VTuple (VCons v1 (VCons v2 VNil))) @ s; E
+     {{{ v, RET v; ⌜ v = v2 ⌝ }}}.
+    Proof.
+      iIntros (ϕ)"_ Hϕ".
+      wp_call.
+      wp_continue.
+      by iApply "Hϕ".
+    Qed.
+  End Stdlib__spec__tuples.
+
 
   (* Lemmas to better handle fully-applied functions of the standart library. *)
   Lemma Stdlib__load__spec_tac vl ℓ v s E :
@@ -224,30 +357,112 @@ Section Stdlib_Lemmas.
   Qed.
 
   Lemma Stdlib__fst__spec_tac s E v v1 v2 ϕ :
-    ⌜ v = VTuple (VCons v1 (VCons v2 VNil)) ⌝ -∗
+    v = VTuple (VCons v1 (VCons v2 VNil)) →
     ▷ ϕ v1 -∗
     WP call Stdlib__fst v @ s; E {{ ϕ }}.
   Proof.
-    iIntros "-> Hϕ".
+    iIntros (->) "Hϕ".
     iApply ((Stdlib__fst__spec v1 v2 s E ϕ) with "[//]").
     iNext. iIntros (?->).
     iAssumption.
   Qed.
 
   Lemma Stdlib__snd__spec_tac s E v v1 v2 ϕ :
-    ⌜ v = VTuple (VCons v1 (VCons v2 VNil)) ⌝ -∗
+    v = VTuple (VCons v1 (VCons v2 VNil)) →
     ▷ ϕ v2 -∗
     WP call Stdlib__snd v @ s; E {{ ϕ }}.
   Proof.
-    iIntros "-> Hϕ".
+    iIntros (->)"Hϕ".
     iApply ((Stdlib__snd__spec v1 v2 s E ϕ) with "[//]").
     iNext. iIntros (?->).
     iAssumption.
   Qed.
+End Stdlib__specs.
 
-End Stdlib_Lemmas.
+Global Opaque Stdlib__mul.
+Global Opaque Stdlib__add.
+Global Opaque Stdlib__add.
+Global Opaque Stdlib__ref.
+Global Opaque Stdlib__load.
+Global Opaque Stdlib__store.
+Global Opaque Stdlib__fst.
+Global Opaque Stdlib__snd.
 
-(* TODO:
-Section Stdlib_tactics.
-  Context `{!osirisGS_gen hlc Σ}.
-End Stdlib_tactics. *)
+
+
+(* -------------------------------------------------------------------------- *)
+
+(* The rest of the file defines a tactic to automatically reduce calls to
+   functions of the standard library. *)
+
+Lemma binop `{!osirisGS_gen hlc Σ} s E :
+  ∀ op (f: Z → Z → val) (i1 i2: Z) φ,
+    let v1 := encode i1 in
+    let v2 := encode i2 in
+    (⊢ WP call op v1 @ s; E
+          {{ λ vpartial, WP call vpartial v2 @ s; E
+                            {{ λ res, ⌜ res  = f i1 i2 ⌝ }} }}) →
+    φ (f i1 i2) -∗
+    WP call op v1 @ s; E {{ λ vpartial,
+                           WP call vpartial v2 @ s; E
+                              {{ φ }} }}.
+Proof.
+  iIntros (op f i1 i2 φ v1 v2 op_spec) "Hφ".
+  iPoseProof op_spec as "Hop_spec".
+  iApply (wp_covariant with "Hop_spec").
+  iIntros (v) "Hv".
+  iApply (wp_covariant with "Hv").
+  iIntros (?->).
+  iExact "Hφ".
+Qed.
+
+
+(* Shadow the standart [wp] tactic to automatically deal with operations. *)
+Ltac wp :=
+  iStartProof; cbn;
+  repeat
+    lazymatch goal with
+    | |- environments.envs_entails _ (▷ _) => iNext
+    | |- environments.envs_entails
+          ?Δ
+          (wp ?s ?E (call Stdlib__fst ?v) ?φ) =>
+        apply (tac_change_goal
+                  Δ _ _
+                  (Stdlib__fst__spec_tac _ _ _ _ _ _ eq_refl));
+        iNext; wp_continue
+    | |- environments.envs_entails
+          ?Δ
+          (wp ?s ?E (call Stdlib__snd ?v) ?φ) =>
+        apply (tac_change_goal
+                  Δ _ _
+                  (Stdlib__snd__spec_tac _ _ _ _ _ _ eq_refl));
+        iNext; wp_continue
+    | |- environments.envs_entails
+          _
+          (wp _ _ (call Stdlib__mul ?v1)
+              (λ vpartial, wp _ _ (call vpartial ?v2) ?φ )) =>
+        apply (tac_change_goal
+                  _ _ _
+                  (binop
+                     _ _ _ (fun i1 i2 => encode (i1 * i2)%Z) _ _ _
+                     (Stdlib__mul__spec _ _ _ _ _ _ eq_refl eq_refl)))
+    | |- environments.envs_entails
+          _
+          (wp _ _ (call Stdlib__sub ?v1)
+              (λ vpartial, wp _ _ (call vpartial ?v2) ?φ )) =>
+        apply (tac_change_goal
+                  _ _ _
+                  (binop
+                     _ _ _ (fun i1 i2 => encode (i1 - i2)%Z) _ _ _
+                     (Stdlib__sub__spec _ _ _ _ _ _ eq_refl eq_refl)))
+    | |- environments.envs_entails
+          _
+          (wp _ _ (call Stdlib__add ?v1)
+              (λ vpartial, wp _ _ (call vpartial ?v2) ?φ )) =>
+        apply (tac_change_goal
+                  _ _ _
+                  (binop
+                     _ _ _ (fun i1 i2 => encode (i1 + i2)%Z) _ _ _
+                     (Stdlib__add__spec _ _ _ _ _ _ eq_refl eq_refl)))
+    | _ => wp_step
+    end.
