test/coq/arith_proof.v
@@ -1,0 +1,177 @@
+From iris.proofmode Require Import base proofmode classes.
+From iris.base_logic.lib Require Import fancy_updates.
+From iris.bi Require Import weakestpre.
+From iris.prelude Require Import options.
+Import uPred.
+
+From osiris Require Import base.
+From osiris.lang Require Import lang.
+From osiris.semantics Require Import semantics.
+From osiris.weakestpre Require Import wp wp_tactics notations.
+From osiris.libs Require Import Stdlib.
+From test Require Import arith.
+
+Context `{!osirisGS_gen hlc Σ}.
+
+Definition add_spec vadd : iProp Σ :=
+  ∀ (x y: Z) (vx vy: val),
+    ⌜ vx = encode x ⌝ -∗
+    ⌜ vy = encode y ⌝ -∗
+    WP call vadd vx
+    {{ λ v, WP call v vy {{ λ res, ⌜res = encode (x + y)%Z⌝ }} }}.
+
+Definition mult_spec vmult : iProp Σ :=
+  ∀ (x: Z),
+    WP call vmult (encode x)
+    {{ λ v, ∀ (y: Z),
+        ⌜ (int.min_signed ≤ x ≤ int.max_signed)%Z⌝ -∗
+        ⌜ (int.min_signed ≤ y ≤ int.max_signed)%Z⌝ -∗
+        WP call v (encode y) {{ λ res, ⌜res = encode (x * y)%Z⌝ }} }}.
+
+Lemma Add_spec :
+    let Λ :=
+    [
+      ("add", add_spec)
+    ]
+  in
+  let η := EnvCons "Stdlib" Stdlib $
+           EnvNil in
+  ⊢ WP eval_mexpr η Arith {{ module_spec Λ }}.
+Proof.
+  intros.
+  wp.
+
+  wp_specify "add" add_spec.
+  { iIntros (x y ??->->).
+    wp_call.
+    do 3 wp_continue.
+
+    wp.
+    do 2 wp_continue.
+
+    wp_par; [ by iApply Stdlib__add__spec
+            | by iApply Stdlib__add__spec | ].
+    iNext. iIntros (v1 v2) "H1 ->".
+    wp_use "H1". }
+  iIntros (v) "#add_spec"; wp_continue.
+
+  wp_specify "mult" mult_spec.
+  { iLöb as "IH".
+    iIntros (x).
+    wp_call.
+    iIntros (y Hx Hy).
+    wp.
+    iApply wp_covariant.
+    { iPoseProof (Stdlib__eq__spec
+                    NotStuck top
+                    (encode y))
+        as "H".
+      4: instantiate (2 := 0%Z).
+      1, 2: exact eq_refl.
+      1: assumption.
+      1: { apply int.prove_representable_30.
+           by vm_compute. }
+      replace (VInt (int.repr y)) with (encode y); last reflexivity.
+      iExact "H". }
+    iIntros (vpartial) "Hpartial". wp.
+    iApply (wp_covariant with "Hpartial").
+    iIntros (vres->).
+    destruct (decide (y = 0)) as [-> | Hneq%Z.eqb_neq].
+    { (* y = 0 *)
+      simpl; wp.
+      iPureIntro.
+      do 2 f_equal. lia. }
+    { (* y <> 0 *)
+      rewrite Hneq. wp.
+      iPoseProof Stdlib__lt__spec as "Hpartial".
+      2 : instantiate (2 := encode 0%Z).
+      1: instantiate (2 := encode y).
+      1,2 : exact eq_refl.
+      2: { apply int.prove_representable_30.
+           by vm_compute. }
+      1: assumption.
+      iApply (wp_covariant with "Hpartial").
+      iIntros (vpartial') "Hpartial'".
+      wp. iApply (wp_covariant with "Hpartial'").
+      iIntros(?->).
+
+      destruct (decide (y < 0)%Z) as [ ->%Z.ltb_lt | n ].
+      { (* y < 0 *)
+        wp.
+        wp_par.
+        2: { iPoseProof (Stdlib__neg__spec) as "H".
+             1: reflexivity.
+             iExact "H". }
+        2: { iNext. iIntros (? ?) "Hpartial' ->".
+             wp. iExact "Hpartial'". }
+        { iSpecialize ("IH" $! x).
+          iApply (wp_covariant with "IH").
+          iIntros (?) "H".
+          iSpecialize ("H" $! (-y)%Z with "[//][]").
+          { (* Prove that -y is reprensentable *) admit. }
+          iApply (wp_covariant with "H").
+          iIntros (?->).
+          iPoseProof Stdlib__neg__spec as "Hneg"; first reflexivity.
+          iApply (wp_covariant with "Hneg").
+          iIntros (?->).
+          iPureIntro.
+          unfold encode, Encode_Z.
+          do 2 f_equal.
+          lia. } }
+      { (* y >= 0 *)
+        apply Z.ltb_nlt in n; rewrite n. wp.
+        iIntros ([]); wp.
+        { (* version without the assertion. *)
+          (* Code: [x + x * (mult x (y -1))]
+             The tree of [Par] is as follows :
+             Par
+               (λ y, x + y) as [ Par [ret _] [ret _] ]
+               (Par
+                  (λ y, x * y) as [ Par [ret _] [ret _] ]
+                  (Par
+                     (λ y, mult x y)
+                     (y - 1))) *)
+
+          wp_par;
+            [ (* [Stdlib__add__spec] is enough to prove the spec of  λ y, x + y *)
+              by iApply Stdlib__add__spec
+            | wp_par;
+              [ (*1: spec of [λ y, mult x y] *)
+              | (*2: spec of [y - 1] *)
+              | (* ... *)]
+            | (*3: proof of [ x * y = x + x * (y - 1)] *)].
+          { wp. (* spec of [mult #x] *)
+            instantiate
+              (1 :=
+                 λ (v: val),
+                 (∀ (y: Z),
+                     ⌜ (int.min_signed ≤ x ≤ int.max_signed)%Z⌝ -∗
+                     ⌜ (int.min_signed ≤ y ≤ int.max_signed)%Z⌝ -∗
+                     WP call v (encode y)
+                        {{ λ res, ⌜res = encode (x * y)%Z⌝ }} )%I).
+            iSpecialize ("IH" $! x).
+            iApply (wp_covariant with "IH").
+            iIntros (?) "?". iAssumption. }
+          { (* spec of [y - 1] *)
+            instantiate (1 := λ v, ⌜v = encode (y-1)%Z⌝%I ).
+            by wp. }
+          { (* spec of [mult x (y-1)] *)
+            iNext. iIntros (v1 v2) "H1 ->".
+            wp.
+            instantiate (1 := λ (v: val), ⌜ v = encode (x * (y - 1))%Z ⌝%I ).
+            iApply "H1"; try done.
+
+            (* Proof that y-1 is representable. *) admit. }
+
+          { iNext. iIntros (v1 v2) "H1 ->".
+            wp.
+            iApply (wp_covariant with "H1").
+            iIntros (?->).
+            iPureIntro; do 2 f_equal. lia. } }
+
+        { (* version with the assertion *) admit. } } } }
+  iIntros (vmult) "#mult_spec"; wp_continue.
+
+  (* All expected specifications have already been proven. *)
+  wp_module_spec.
+Admitted.
